Wavelet/Lemmas.lean
@@ -26,6 +26,16 @@ theorem mapM_some_iff_forall₂
 
 end List
 
+namespace Array
+
+@[simp]
+theorem mapM_push [Monad m] [LawfulMonad m] {f : α → m β} {xs : Array α} :
+    (xs.push x).mapM f = (return (← xs.mapM f).push (← f x)) := by
+  rcases xs with ⟨xs⟩
+  simp
+
+end Array
+
 namespace Vector
 
 theorem mapM_some_implies_all_some {α β} {f : α → Option β} {xs : Vector α n} {ys : Vector β n} :
@@ -36,6 +46,38 @@ theorem mapM_some_implies_all_some {α β} {f : α → Option β} {xs : Vector �
 theorem mapM_toList {α β} {f : α → Option β} {xs : Vector α n} {ys : Vector β n}
   (h : Vector.mapM f xs = some ys):
   List.mapM f xs.toList = some ys.toList
+:= sorry
+
+theorem mapM_push [Monad m] [LawfulMonad m]
+  {f : α → m β} {xs : Vector α n} :
+  (xs.push x).mapM f = (return (← xs.mapM f).push (← f x))
+:= by
+  apply map_toArray_inj.mp
+  suffices toArray <$> (xs.push x).mapM f = (return (← toArray <$> xs.mapM f).push (← f x)) by
+    rw [this]
+    simp only [bind_pure_comp, Functor.map_map, bind_map_left, map_bind, toArray_push]
+  simp
+
+theorem mem_pop_implies_mem
+  {xs : Vector α (n + 1)}
+  (h : x ∈ xs.pop) : x ∈ xs
+:= sorry
+
+theorem mem_pop_iff
+  {xs : Vector α (n + 1)} :
+  x ∈ xs ↔ x ∈ xs.pop ∨ x = xs.back
+:= sorry
+
+theorem nodup_implies_pop_nodup
+  {xs : Vector α (n + 1)}
+  (h : xs.toList.Nodup) :
+  xs.pop.toList.Nodup
+:= sorry
+
+theorem nodup_implies_back_not_mem_pop
+  {xs : Vector α (n + 1)}
+  (h : xs.toList.Nodup) :
+  xs.back ∉ xs.pop
 := sorry
 
 end Vector
